zoo_saturn/spmc_queue: Verify.

theories/zoo_saturn/spmc_queue.v
@@ -4,6 +4,7 @@ From iris.base_logic Require Import
 From zoo Require Import
   prelude.
 From zoo.common Require Import
+  relations
   countable
   list.
 From zoo.iris.bi Require Import
@@ -104,6 +105,11 @@ Section spmc_queue_G.
   #[local] Definition front_lb γ i :=
     auth_nat_max_lb γ.(metadata_front) i.
 
+  #[local] Definition producer' γ_model ws :=
+    auth_twins_auth _ γ_model ws.
+  #[local] Definition producer γ :=
+    producer' γ.(metadata_model).
+
   #[local] Definition model₁' γ_model vs :=
     auth_twins_twin1 _ γ_model vs.
   #[local] Definition model₁ γ :=
@@ -112,11 +118,6 @@ Section spmc_queue_G.
     auth_twins_twin2 _ γ_model vs.
   #[local] Definition model₂ γ :=
     model₂' γ.(metadata_model).
-
-  #[local] Definition producer' γ_model ws :=
-    auth_twins_auth _ γ_model ws.
-  #[local] Definition producer γ :=
-    producer' γ.(metadata_model).
 
   #[local] Definition waiters_auth' γ_waiters waiters :=
     ghost_map_auth γ_waiters 1 waiters.
@@ -143,11 +144,9 @@ Section spmc_queue_G.
       waiter_au γ ι Ψ.
 
   #[local] Definition inv_inner l γ ι : iProp Σ :=
-    ∃ hist past front nodes back vs waiters,
+    ∃ hist past front nodes vs waiters,
     ⌜hist = past ++ front :: nodes⌝ ∗
-    ⌜back ∈ hist⌝ ∗
     l.[front] ↦ #front ∗
-    l.[back] ↦ #back ∗
     xtchain (Header §Node 2) (DfracOwn 1) hist §Null ∗
     ([∗ list] node; v ∈ nodes; vs, node.[xtchain_data] ↦ v) ∗
     history_auth γ hist ∗
@@ -161,13 +160,10 @@ Section spmc_queue_G.
       %past{} &
       %front{} &
       %nodes{} &
-      %back{} &
       %vs{} &
       %waiters{} &
       >%Hhist{} &
-      >%Hback{} &
       >Hl_front &
-      >Hl_back &
       >Hhist &
       >Hnodes &
       >Hhistory_auth &
@@ -190,6 +186,27 @@ Section spmc_queue_G.
       #Hinv
     )".
 
+  Definition spmc_queue_producer t ws : iProp Σ :=
+    ∃ l γ back,
+    ⌜t = #l⌝ ∗
+    meta l nroot γ ∗
+    l.[back] ↦ #back ∗
+    back ↦ₕ Header §Node 2 ∗
+    history_last γ back ∗
+    producer γ ws.
+  #[local] Instance : CustomIpatFormat "producer" :=
+    "(
+      %l_{} &
+      %γ_{} &
+      %back{} &
+      %Heq{} &
+      #Hmeta_{} &
+      Hl_back{_{}} &
+      #Hback{}_header &
+      Hhistory_last{_{}} &
+      Hproducer{_{}}
+    )".
+
   Definition spmc_queue_model t vs : iProp Σ :=
     ∃ l γ,
     ⌜t = #l⌝ ∗
@@ -197,27 +214,11 @@ Section spmc_queue_G.
     model₁ γ vs.
   #[local] Instance : CustomIpatFormat "model" :=
     "(
-      %l_ &
-      %γ_ &
-      %Heq &
-      #Hmeta_ &
-      Hmodel₁
-    )".
-
-  Definition spmc_queue_producer t ws : iProp Σ :=
-    ∃ l γ back,
-    ⌜t = #l⌝ ∗
-    meta l nroot γ ∗
-    l.[back] ↦ #back ∗
-    history_last γ back ∗
-    producer γ ws.
-  #[local] Instance : CustomIpatFormat "producer" :=
-    "(
-      %l{{}=_} &
-      %γ{{}=_} &
+      %l_{} &
+      %γ_{} &
       %Heq{} &
       #Hmeta_{} &
-      Hmodel₁{}
+      Hmodel₁
     )".
 
   #[global] Instance spmc_queue_model_timeless t vs :
@@ -236,20 +237,183 @@ Section spmc_queue_G.
     apply _.
   Qed.
 
+  #[local] Lemma history_alloc front :
+    ⊢ |==>
+      ∃ γ_history,
+      history_auth' γ_history [front] ∗
+      history_last' γ_history front.
+  Proof.
+    iMod mono_list_alloc as "(%γ_history & $ & $)".
+    iSteps.
+  Qed.
+  #[local] Lemma history_at_get {γ hist} i node :
+    hist !! i = Some node →
+    history_auth γ hist ⊢
+    history_at γ i node.
+  Proof.
+    apply mono_list_at_get.
+  Qed.
+  #[local] Lemma history_agree γ hist i node :
+    history_auth γ hist -∗
+    history_at γ i node -∗
+    ⌜hist !! i = Some node⌝.
+  Proof.
+    apply mono_list_at_valid.
+  Qed.
+  #[local] Lemma history_auth_last γ hist node :
+    history_auth γ hist -∗
+    history_last γ node -∗
+    ⌜last hist = Some node⌝.
+  Proof.
+    iIntros "Hauth_1 (:history_last =2)".
+    iDestruct (mono_list_auth_agree with "Hauth_1 Hauth_2") as %<-.
+    iSteps.
+  Qed.
+  #[local] Lemma history_update {γ hist node} node' :
+    history_auth γ hist -∗
+    history_last γ node ==∗
+      history_auth γ (hist ++ [node']) ∗
+      history_last γ node'.
+  Proof.
+    iIntros "Hauth_1 (:history_last =2)".
+    rewrite /history_auth /history_auth'.
+    iDestruct (mono_list_auth_combine with "Hauth_1 Hauth_2") as "(<- & Hauth)". rewrite dfrac_op_own Qp.half_half.
+    iMod (mono_list_update_snoc with "Hauth") as "($ & $)".
+    rewrite last_snoc //.
+  Qed.
+
+  #[local] Lemma front_alloc :
+    ⊢ |==>
+      ∃ γ_front,
+      front_auth' γ_front 0.
+  Proof.
+    apply auth_nat_max_alloc.
+  Qed.
+  #[local] Lemma front_lb_get γ i :
+    front_auth γ i ⊢
+    front_lb γ i.
+  Proof.
+    apply auth_nat_max_lb_get.
+  Qed.
+  #[local] Lemma front_lb_valid γ i1 i2 :
+    front_auth γ i1 -∗
+    front_lb γ i2 -∗
+    ⌜i2 ≤ i1⌝.
+  Proof.
+    apply auth_nat_max_lb_valid.
+  Qed.
+  #[local] Lemma front_update {γ i} i' :
+    i ≤ i' →
+    front_auth γ i ⊢ |==>
+    front_auth γ i'.
+  Proof.
+    apply auth_nat_max_update.
+  Qed.
+
+  #[local] Lemma producer_valid_1 γ ws vs :
+    producer γ ws -∗
+    model₁ γ vs -∗
+    ⌜vs `suffix_of` ws⌝.
+  Proof.
+    rewrite -preorder_rtc.
+    apply: auth_twins_valid_1.
+  Qed.
+  #[local] Lemma producer_exclusive γ ws1 ws2 :
+    producer γ ws1 -∗
+    producer γ ws2 -∗
+    False.
+  Proof.
+    apply: auth_twins_auth_exclusive.
+  Qed.
+
+  #[local] Lemma model_producer_alloc :
+    ⊢ |==>
+      ∃ γ_model,
+      producer' γ_model [] ∗
+      model₁' γ_model [] ∗
+      model₂' γ_model [].
+  Proof.
+    apply auth_twins_alloc.
+  Qed.
+  #[local] Lemma model_agree γ vs1 vs2 :
+    model₁ γ vs1 -∗
+    model₂ γ vs2 -∗
+    ⌜vs1 = vs2⌝.
+  Proof.
+    apply: auth_twins_agree_L.
+  Qed.
+  #[local] Lemma model_push {γ ws vs1 vs2} v :
+    producer γ ws -∗
+    model₁ γ vs1 -∗
+    model₂ γ vs2 ==∗
+      producer γ (vs1 ++ [v]) ∗
+      model₁ γ (vs1 ++ [v]) ∗
+      model₂ γ (vs1 ++ [v]).
+  Proof.
+    apply auth_twins_update_auth.
+  Qed.
+  #[local] Lemma model_pop γ v vs1 vs2 :
+    model₁ γ (v :: vs1) -∗
+    model₂ γ vs2 ==∗
+      model₁ γ vs1 ∗
+      model₂ γ vs1.
+  Proof.
+    apply: auth_twins_update_twins_L.
+    rewrite preorder_rtc. solve_suffix.
+  Qed.
+
+  #[local] Lemma waiters_alloc :
+    ⊢ |==>
+      ∃ γ_waiters,
+      waiters_auth' γ_waiters ∅.
+  Proof.
+    iMod ghost_map_alloc as "(%γ_waiters & Hwaiters_auth & _)".
+    iSteps.
+  Qed.
+  #[local] Lemma waiters_lookup γ waiters waiter i :
+    waiters_auth γ waiters -∗
+    waiters_at γ waiter i -∗
+    ⌜waiters !! waiter = Some i⌝.
+  Proof.
+    apply ghost_map_lookup.
+  Qed.
+  #[local] Lemma waiters_insert {γ waiters} waiter i :
+    waiters !! waiter = None →
+    waiters_auth γ waiters ⊢ |==>
+      waiters_auth γ (<[waiter := i]> waiters) ∗
+      waiters_at γ waiter i.
+  Proof.
+    iIntros "%Hlookup Hwaiters_auth".
+    iApply (ghost_map_insert with "Hwaiters_auth"); first done.
+  Qed.
+  #[local] Lemma waiters_delete γ waiters waiter i :
+    waiters_auth γ waiters -∗
+    waiters_at γ waiter i ==∗
+    waiters_auth γ (delete waiter waiters).
+  Proof.
+    apply ghost_map_delete.
+  Qed.
+
   Opaque history_last'.
 
   Lemma spmc_queue_producer_valid t vs ws :
-    spmc_queue_model t vs -∗
     spmc_queue_producer t ws -∗
+    spmc_queue_model t vs -∗
     ⌜vs `suffix_of` ws⌝.
   Proof.
-  Admitted.
+    iIntros "(:producer =1) (:model =2)". simplify.
+    iDestruct (meta_agree with "Hmeta_1 Hmeta_2") as %->.
+    iApply (producer_valid_1 with "Hproducer_1 Hmodel₁").
+  Qed.
   Lemma spmc_queue_producer_exclusive t ws1 ws2 :
     spmc_queue_producer t ws1 -∗
     spmc_queue_producer t ws2 -∗
     False.
   Proof.
-  Admitted.
+    iIntros "(:producer =1) (:producer =2)". simplify.
+    iDestruct (meta_agree with "Hmeta_1 Hmeta_2") as %->.
+    iApply (producer_exclusive with "Hproducer_1 Hproducer_2").
+  Qed.
 
   Lemma spmc_queue_create_spec ι :
     {{{
@@ -263,7 +427,238 @@ Section spmc_queue_G.
       spmc_queue_producer t []
     }}}.
   Proof.
-  Admitted.
+    iIntros "%Φ _ HΦ".
+
+    wp_rec.
+
+    wp_block front as "#Hfront_header" "_" "(Hfront_next & _)".
+    wp_block l as "Hmeta" "(Hl_front & Hl_back & _)".
+
+    iMod history_alloc as "(%γ_history & Hhistory_auth & Hhistory_last)".
+    iMod front_alloc as "(%γ_front & Hfront_auth)".
+    iMod model_producer_alloc as "(%γ_model & Hproducer & Hmodel₁ & Hmodel₂)".
+    iMod waiters_alloc as "(%γ_waiters & Hwaiters_auth)".
+
+    pose γ := {|
+      metadata_history := γ_history ;
+      metadata_front := γ_front ;
+      metadata_model := γ_model ;
+      metadata_waiters := γ_waiters ;
+    |}.
+
+    iMod (meta_set γ with "Hmeta") as "#Hmeta"; first done.
+
+    iApply "HΦ".
+    iSplitR "Hmodel₁ Hl_back Hhistory_last Hproducer"; last iSteps.
+    iStep 2. iApply inv_alloc.
+    iExists [front], [], front, [], [], ∅. iFrameSteps.
+    rewrite xtchain_singleton big_sepM_empty. iSteps.
+  Qed.
+
+  #[local] Lemma front_spec_strong au Ψ l γ ι :
+    {{{
+      inv ι (inv_inner l γ ι) ∗
+      if negb au then True else
+        waiter_au γ ι Ψ
+    }}}
+      (#l).{front}
+    {{{ front i,
+      RET #front;
+      front ↦ₕ Header §Node 2 ∗
+      history_at γ i front ∗
+      front_lb γ i ∗
+      if negb au then True else
+        ∃ waiter,
+        saved_pred waiter Ψ ∗
+        waiters_at γ waiter i
+    }}}.
+  Proof.
+    iIntros "%Φ (#Hinv & HΨ) HΦ".
+
+    iInv "Hinv" as "(:inv_inner)".
+    wp_load.
+    assert (hist !! (length past) = Some front) as Hlookup.
+    { rewrite Hhist list_lookup_middle //. }
+    iDestruct (xtchain_lookup_header with "Hhist") as "#Hfront_header"; first done.
+    iDestruct (history_at_get _ front with "Hhistory_auth") as "#Hhistory_at"; first done.
+    iDestruct (front_lb_get with "Hfront_auth") as "#Hfront_lb".
+    destruct au; last iSteps.
+    iMod (saved_pred_alloc_cofinite (dom waiters) Ψ) as "(%waiter & %Hwaiter & #Hwaiter)".
+    rewrite not_elem_of_dom in Hwaiter.
+    iMod (waiters_insert _ (length past) with "Hwaiters_auth") as "(Hwaiter_auth & Hwaiters_at)"; first done.
+    iDestruct (big_sepM_insert_2 _ _ waiter (length past) with "[HΨ] Hwaiters") as "Hwaiters".
+    { iExists Ψ. rewrite decide_False; first lia. iSteps. }
+    iSplitR "Hwaiters_at HΦ". { iFrameSteps. }
+    iSteps.
+  Qed.
+  #[local] Lemma front_spec l γ ι :
+    {{{
+      inv ι (inv_inner l γ ι)
+    }}}
+      (#l).{front}
+    {{{ front i,
+      RET #front;
+      front ↦ₕ Header §Node 2 ∗
+      history_at γ i front ∗
+      front_lb γ i
+    }}}.
+  Proof.
+    iIntros "%Φ #Hinv HΦ".
+    wp_apply (front_spec_strong false inhabitant with "[$Hinv]").
+    iSteps.
+  Qed.
+
+  Inductive op :=
+    | IsEmpty
+    | Pop
+    | Other.
+  #[local] Instance op_eq_dec : EqDecision op :=
+    ltac:(solve_decision).
+  #[local] Lemma xtchain_next_spec_strong op TB waiter Ψ_is_empty β x Ψ_pop l γ ι i node :
+    {{{
+      meta l nroot γ ∗
+      inv ι (inv_inner l γ ι) ∗
+      history_at γ i node ∗
+      ( if decide (op = Other) then True else
+          front_lb γ i
+      ) ∗
+      match op with
+      | IsEmpty =>
+          saved_pred waiter Ψ_is_empty ∗
+          waiters_at γ waiter i ∗
+          £ 1
+      | Pop =>
+          atomic_update (TA := [tele vs]) (TB := TB) (⊤ ∖ ↑ι) ∅ (tele_app $ spmc_queue_model #l) β Ψ_pop ∗
+          (spmc_queue_model #l [] -∗ β [tele_arg []] x)
+      | Other =>
+          True
+      end
+    }}}
+      (#node).{xtchain_next}
+    {{{ res,
+      RET res;
+      ( ⌜res = ()%V⌝ ∗
+        match op with
+        | IsEmpty =>
+            Ψ_is_empty true
+        | Pop =>
+            Ψ_pop [tele_arg []] x
+        | Other =>
+            True
+        end
+      ) ∨ (
+        ∃ node',
+        ⌜res = #node'⌝ ∗
+        node' ↦ₕ Header §Node 2 ∗
+        history_at γ (S i) node' ∗
+        match op with
+        | IsEmpty =>
+            Ψ_is_empty false
+        | Pop =>
+            atomic_update (TA := [tele vs]) (TB := TB) (⊤ ∖ ↑ι) ∅ (tele_app $ spmc_queue_model #l) β Ψ_pop
+        | Other =>
+            True
+        end
+      )
+    }}}.
+  Proof.
+    iIntros "%Φ (#Hmeta & #Hinv & #Hhistory_at & Hop) HΦ".
+
+    iInv "Hinv" as "(:inv_inner)".
+    iDestruct (history_agree with "Hhistory_auth Hhistory_at") as %Hlookup.
+    iDestruct (xtchain_lookup_acc with "Hhist") as "(_ & Hnode & Hhist)"; first done.
+    wp_load.
+    iDestruct ("Hhist" with "Hnode ") as "Hhist".
+    destruct (hist !! S i) as [node' |] eqn:Hlookup'; simpl.
+
+    - iDestruct (xtchain_lookup_header with "Hhist") as "#Hnode'_header"; first done.
+      iDestruct (history_at_get (S i) with "Hhistory_auth") as "#Hhistory_at'"; first done.
+      destruct op; [| iSteps..].
+      iDestruct "Hop" as "(#Hfront_lb & #Hwaiter & Hwaiters_at & H£)".
+      iDestruct (waiters_lookup with "Hwaiters_auth Hwaiters_at") as %Hwaiters_lookup.
+      iMod (waiters_delete with "Hwaiters_auth Hwaiters_at") as "Hwaiters_auth".
+      iDestruct (big_sepM_delete with "Hwaiters") as "((%Ψ & _Hwaiter & HΨ) & Hwaiters)"; first done.
+      iDestruct (saved_pred_agree false with "Hwaiter _Hwaiter") as "HΨ_is_empty".
+      iMod (lc_fupd_elim_later with "H£ HΨ_is_empty") as "HΨ_is_empty".
+      destruct (decide (i = length past)) as [-> | Hi].
+
+      + rewrite decide_False; first lia.
+        iMod "HΨ" as "(%_vs & Hmodel₁ & _ & HΨ)".
+        iDestruct (model_agree with "Hmodel₁ Hmodel₂") as %->.
+        iMod ("HΨ" with "Hmodel₁") as "HΨ".
+        assert (nodes ≠ []) as Hnodes.
+        { apply lookup_lt_Some in Hlookup'.
+          rewrite Hhist length_app /= in Hlookup'.
+          naive_solver lia.
+        }
+        iAssert ⌜vs ≠ []⌝%I as %Hvs.
+        { destruct (decide (vs = [])) as [-> |]; last done.
+          iDestruct (big_sepL2_length with "Hnodes") as %->%nil_length_inv.
+          iSteps.
+        }
+        rewrite bool_decide_eq_false_2 //.
+        iSplitR "HΨ_is_empty HΨ HΦ". { iFrameSteps. }
+        iSteps. iRewrite "HΨ_is_empty". iSteps.
+
+      + iDestruct (front_lb_valid with "Hfront_auth Hfront_lb") as %Hi_.
+        rewrite decide_True; first lia.
+        iSplitR "HΨ_is_empty HΨ HΦ". { iFrameSteps. }
+        iSteps. iRewrite "HΨ_is_empty". iSteps.
+
+    - destruct (decide (op = Other)) as [-> | Hop]; first iSteps.
+      iDestruct "Hop" as "(#Hfront_lb & Hop)".
+      iDestruct (front_lb_valid with "Hfront_auth Hfront_lb") as %Hi.
+      opose proof* length_lookup_last as Hlength; [done.. |].
+      rewrite Hhist length_app /= in Hlength.
+      assert (i = length past) as -> by lia.
+      assert (length nodes = 0) as ->%nil_length_inv by lia.
+      iDestruct (big_sepL2_length with "Hnodes") as %->%symmetry%nil_length_inv.
+      destruct op; last done.
+
+      + iDestruct "Hop" as "(#Hwaiter & Hwaiters_at & H£)".
+        iDestruct (waiters_lookup with "Hwaiters_auth Hwaiters_at") as %Hwaiters_lookup.
+        iMod (waiters_delete with "Hwaiters_auth Hwaiters_at") as "Hwaiters_auth".
+        iDestruct (big_sepM_delete with "Hwaiters") as "((%Ψ & _Hwaiter & HΨ) & Hwaiters)"; first done.
+        iDestruct (saved_pred_agree true with "Hwaiter _Hwaiter") as "HΨ_is_empty".
+        iMod (lc_fupd_elim_later with "H£ HΨ_is_empty") as "HΨ_is_empty".
+        rewrite decide_False; first lia.
+        iMod "HΨ" as "(%vs & Hmodel₁ & _ & HΨ)".
+        iDestruct (model_agree with "Hmodel₁ Hmodel₂") as %->.
+        iMod ("HΨ" with "Hmodel₁") as "HΨ".
+        iSplitR "HΨ_is_empty HΨ HΦ". { iFrameSteps. }
+        iModIntro. clear.
+
+        iApply "HΦ".
+        iLeft. iRewrite "HΨ_is_empty". iSteps.
+
+      + iDestruct "Hop" as "(HΨ & Hβ)".
+        iMod "HΨ" as "(%vs & (:model) & _ & HΨ)". injection Heq as <-.
+        iDestruct (meta_agree with "Hmeta Hmeta_") as %<-. iClear "Hmeta_".
+        iDestruct (model_agree with "Hmodel₁ Hmodel₂") as %->.
+        iDestruct ("Hβ" with "[Hmodel₁]") as "Hβ"; first iSteps.
+        iMod ("HΨ" with "Hβ") as "HΨ".
+        iSplitR "HΨ HΦ". { iFrameSteps. }
+        iSteps.
+  Qed.
+  #[local] Lemma xtchain_next_spec l γ ι i node :
+    {{{
+      meta l nroot γ ∗
+      inv ι (inv_inner l γ ι) ∗
+      history_at γ i node
+    }}}
+      (#node).{xtchain_next}
+    {{{ res,
+      RET res;
+        ⌜res = ()%V⌝
+      ∨ ∃ node',
+        ⌜res = #node'⌝ ∗
+        node' ↦ₕ Header §Node 2 ∗
+        history_at γ (S i) node'
+    }}}.
+  Proof.
+    iIntros "%Φ (#Hmeta & #Hinv & #Hhistory_at) HΦ".
+    wp_apply (xtchain_next_spec_strong Other TeleO inhabitant inhabitant inhabitant inhabitant inhabitant); iSteps.
+  Qed.
 
   Lemma spmc_queue_is_empty_spec t ι :
     <<<
@@ -278,7 +673,18 @@ Section spmc_queue_G.
       True
     >>>.
   Proof.
-  Admitted.
+    iIntros "%Φ (:inv) HΦ".
+
+    wp_rec credit:"H£".
+    wp_smart_apply (front_spec_strong true (λ b, Φ #b) with "[$Hinv HΦ]") as (node i) "(#Hnode_header & #Hhistory_at & #Hfront_lb & %waiter & #Hwaiter & Hwaiters_at)".
+    { rewrite /= /waiter_au. iAuIntro.
+      iApply (aacc_aupd_commit with "HΦ"); first done. iIntros "%vs (:model)". injection Heq as <-.
+      iDestruct (meta_agree with "Hmeta Hmeta_") as %<-. iClear "Hmeta_".
+      iAaccIntro with "Hmodel₁"; iSteps.
+    }
+    wp_match.
+    wp_smart_apply (xtchain_next_spec_strong IsEmpty [tele_pair bool] _ _ inhabitant [tele_arg true] inhabitant with "[$Hmeta $Hinv $Hhistory_at $Hfront_lb $Hwaiter $Hwaiters_at $H£]") as (res) "[(-> & HΦ) | (%node' & -> & #Hhistory_at' & HΦ)]"; iSteps.
+  Qed.
 
   Lemma spmc_queue_push_spec t ι ws v :
     <<<
@@ -294,7 +700,30 @@ Section spmc_queue_G.
       spmc_queue_producer t (vs ++ [v])
     >>>.
   Proof.
-  Admitted.
+    iIntros "%Φ ((:inv) & (:producer)) HΦ". injection Heq as <-.
+    iDestruct (meta_agree with "Hmeta Hmeta_") as %<-. iClear "Hmeta_".
+
+    wp_rec.
+    wp_block new_back as "#Hnew_back_header" "_" "(Hnew_back_next & Hnew_back_data & _)".
+    wp_match. wp_load. wp_match.
+
+    wp_bind (_ <-{next} _)%E.
+    iInv "Hinv" as "(:inv_inner)".
+    iDestruct (history_auth_last with "Hhistory_auth Hhistory_last") as %?.
+    wp_apply (xtchain_set_next_spec_last' with "[$Hhist $Hnew_back_next $Hnew_back_header]") as "Hhist"; first done.
+    iMod (history_update new_back with "Hhistory_auth Hhistory_last") as "(Hhistory_auth & Hhistory_last)".
+    iDestruct (big_sepL2_snoc_2 with "Hnodes Hnew_back_data") as "Hnodes".
+
+    iMod "HΦ" as "(%vs_ & (:model) & _ & HΦ)". injection Heq as <-.
+    iDestruct (meta_agree with "Hmeta Hmeta_") as %<-. iClear "Hmeta_".
+    iDestruct (model_agree with "Hmodel₁ Hmodel₂") as %->.
+    iMod (model_push v with "Hproducer Hmodel₁ Hmodel₂") as "(Hproducer & Hmodel₁ & Hmodel₂)".
+    iMod ("HΦ" with "[Hmodel₁]") as "HΦ"; first iSteps.
+
+    iSplitR "Hl_back Hhistory_last Hproducer HΦ".
+    { iFrameSteps. list_simplifier. done. }
+    iSteps.
+  Qed.
 
   Lemma spmc_queue_pop_spec t ι :
     <<<
@@ -309,7 +738,62 @@ Section spmc_queue_G.
       True
     >>>.
   Proof.
-  Admitted.
+    iIntros "%Φ (:inv) HΦ".
+
+    iLöb as "HLöb".
+
+    wp_rec.
+    wp_smart_apply (front_spec with "Hinv") as (front i) "(#Hfront_header & #Hhistory_at & #Hfront_lb)".
+    wp_match.
+    wp_smart_apply (xtchain_next_spec_strong Pop _ inhabitant inhabitant _ [tele_arg] with "[$Hmeta $Hinv $Hhistory_at $Hfront_lb $HΦ]") as (res) "[(-> & HΦ) | (%new_front & -> & #Hnew_front_header & #Hhistory_at_new & HΦ)]"; [iSteps.. |].
+    wp_match. wp_pures.
+
+    wp_bind (CAS _ _ _).
+    iInv "Hinv" as "(:inv_inner =1)".
+    iDestruct (history_agree with "Hhistory_auth Hhistory_at_new") as %Hlookup.
+    iDestruct (xtchain_lookup_acc with "Hhist") as "(_ & Hnode & Hhist)"; first done.
+    wp_cas as _ | [= <-]; first iSteps.
+    iDestruct ("Hhist" with "Hnode ") as "Hhist".
+    iDestruct (history_agree with "Hhistory_auth Hhistory_at") as %Hlookup_old.
+    iAssert ⌜length past1 = i⌝%I as %Hpast_length.
+    { iDestruct (xtchain_NoDup with "Hhist") as %Hnodup.
+      iPureIntro. eapply NoDup_lookup; try done.
+      rewrite Hhist1 list_lookup_middle //.
+    }
+    rewrite Hhist1 (assoc _ _ [_]) lookup_app_r length_app /= in Hlookup; first lia.
+    rewrite Nat.add_1_r Hpast_length Nat.sub_diag in Hlookup.
+    destruct nodes1 as [| node nodes1]; first done. injection Hlookup as ->.
+    rewrite (assoc _ _ [_]) in Hhist1.
+    iDestruct (big_sepL2_cons_inv_l with "Hnodes") as "(%v & %vs' & -> & Hfront_data & Hnodes)".
+    set past := past1 ++ [front].
+    iMod (front_update (length past) with "Hfront_auth") as "Hfront_auth".
+    { rewrite /past. simpl_length. lia. }
+    iDestruct (big_sepM_impl_thread_fupd _ (waiter_model γ ι past)%I with "Hwaiters Hmodel₂ [#]") as ">(Hwaiters & Hmodel₂)".
+    { iIntros "!> %waiter %j %Hlookup (%P & #Hwaiter & HP) Hmodel₂".
+      destruct (Nat.lt_trichotomy j (length past1)) as [Hj | [-> | Hj]].
+      - rewrite decide_True //.
+        rewrite /waiter_model. setoid_rewrite decide_True; last first.
+        { rewrite /past. simpl_length. lia. }
+        iSteps.
+      - rewrite decide_False; first lia.
+        rewrite /waiter_model. setoid_rewrite decide_True; last first.
+        { rewrite /past. simpl_length/=. lia. }
+        iMod "HP" as "(%vs & Hmodel₁ & _ & HP)".
+        iDestruct (model_agree with "Hmodel₁ Hmodel₂") as %->.
+        iSteps.
+      - rewrite decide_False; first lia.
+        rewrite /waiter_model. setoid_rewrite decide_False; last first.
+        { rewrite /past. simpl_length/=. lia. }
+        iSteps.
+    }
+    iMod "HΦ" as "(%_vs & (:model) & _ & HΦ)". injection Heq as <-.
+    iDestruct (meta_agree with "Hmeta Hmeta_") as %<-. iClear "Hmeta_".
+    iDestruct (model_agree with "Hmodel₁ Hmodel₂") as %->.
+    iMod (model_pop with "Hmodel₁ Hmodel₂") as "(Hmodel₁ & Hmodel₂)".
+    iMod ("HΦ" with "[Hmodel₁]") as "HΦ"; first iSteps.
+    iSplitR "Hfront_data HΦ". { iFrameSteps. }
+    iSteps.
+  Qed.
 End spmc_queue_G.
 
 #[global] Opaque spmc_queue_create.
@@ -318,5 +802,5 @@ End spmc_queue_G.
 #[global] Opaque spmc_queue_pop.
 
 #[global] Opaque spmc_queue_inv.
-#[global] Opaque spmc_queue_model.
 #[global] Opaque spmc_queue_producer.
+#[global] Opaque spmc_queue_model.
